Veritas.Verifier.Thread.fst
@@ -49,8 +49,7 @@ let lemma_requires_key_in_store
 let lemma_hadd_correct (tl: verifiable_log):
   Lemma (hadd tl = ms_hashfn (blum_add_seq tl)) = admit()
 
-
-let blum_evict_elem (tl: verifiable_log) (i:idx tl{is_evict_to_blum (index tl i)}): ms_hashfn_dom =
+let blum_evict_elem (tl: verifiable_log) (i:idx tl{is_evict_to_blum (index tl i)}): ms_hashfn_dom =  
   admit()
 
 let blum_evict_seq (tl: verifiable_log): S.seq ms_hashfn_dom = admit()
